\documentclass[14pt]{extarticle}
\usepackage{amsmath}
\usepackage{amssymb}
\usepackage{gvv}
\usepackage{graphicx}
\usepackage{multicol}
\title{\textbf{2.10.34}}
\author{\textbf{Aditya Mishra-EE25BTECH11005}}
\date{October 11, 2025}

\begin{document}
\maketitle

\section*{Question}
Let $\vec{a} = \mathbf{i} - \mathbf{j}$, $\vec{b} = \mathbf{j} - \mathbf{k}$, $\vec{c} = \mathbf{k} - \mathbf{i}$.  
If $\vec{d}$ is a unit vector such that $\vec{a} \cdot \vec{d} = 0 = [\vec{b}~\vec{c}~\vec{d}]$,  
then $\vec{d}$ equals

\begin{multicols}{2}
\begin{enumerate}
    \item $\pm \frac{{\vec{i} + \vec{j} - 2\vec{k}}}{\sqrt{6}}$
    \item $\pm \frac{{\vec{i} + \vec{j} + \vec{k}}}{\sqrt{3}}$
    \item $\pm \frac{{\vec{i} + \vec{j} - \vec{k}}}{\sqrt{3}}$
    \item $\pm {\vec{i} + \vec{j} - \vec{k}}$
\end{enumerate}
\end{multicols}

\section*{Solution}

Given:
\begin{equation}
[\vec{b}~\vec{c}~\vec{d}] = 0
\end{equation}
This implies $\vec{d}$ is linearly dependant on $\vec{b}$ and $\vec{c}$
\begin{equation}
\implies \vec{d} = k\myvec{\vec{b} \ \vec{c}}\myvec{\lambda \\ 1}
\end{equation}
Now, since $\vec{a}^T \vec{d} = 0$,
\begin{align}
k\vec{a}^T (\vec{c} + \lambda \vec{b}) = 0 \\
\implies \vec{a}^T \vec{c} + \lambda \vec{a}^T \vec{b} = 0
\end{align}
\begin{equation}
\lambda = -\frac{\vec{a}^T \vec{c}}{\vec{a}^T \vec{b}}
\end{equation}
Substitute this value of $\lambda$ back:
\begin{equation}
\vec{d} = k(\vec{c} - \frac{\vec{a}^T \vec{c}}{\vec{a}^T \vec{b}} \vec{b})
\end{equation}
To find k:
\begin{equation}
\|\vec{d}|\ = 1
\end{equation}
\begin{equation}
k = \pm \frac{1}{\|\vec{c} - \frac{\vec{a}^T \vec{c}}{\vec{a}^T \vec{b}} \vec{b}\|}
\end{equation}

\begin{equation}
    \vec{d} = \pm \frac{(\vec{c} - \frac{\vec{a}^T \vec{c}}{\vec{a}^T \vec{b}} \vec{b})}{\|\vec{c} - \frac{\vec{a}^T \vec{c}}{\vec{a}^T \vec{b}} \vec{b}\|}
\end{equation}

\section*{Substituting Numbers}

Given:
\begin{align}
\vec{a} = \mathbf{i} - \mathbf{j}, \quad \vec{b} = \mathbf{j} - \mathbf{k}, \quad \vec{c} = \mathbf{k} - \mathbf{i}
\end{align}
So,
\begin{equation}
\vec{d} = \pm \frac{\mathbf{i} + \mathbf{j} - 2\mathbf{k}}{\sqrt{6}}
\end{equation}

\section*{Answer: Option 1}
\[
\boxed{
\vec{d} = \pm \frac{\mathbf{i} + \mathbf{j} - 2\mathbf{k}}{\sqrt{6}}
}
\]

\end{document}

